byteback-core/src/main/java/byteback/core/converter/soottoboogie/method/procedure/ProcedureConversionException.java
@@ -19,8 +19,7 @@ public class ProcedureConversionException extends ConversionException {
 
 	@Override
 	public String getMessage() {
-
-		return "Exception while converting procedure method " + method.getIdentifier() + ":\n" + super.getMessage();
+		return "While converting procedure method " + method.getIdentifier() + ":\n" + super.getMessage();
 	}
 
 }
