byteback-dummy/java8/src/main/java/byteback/dummy/invalid/Assertions.java
@@ -1,0 +1,9 @@
+package byteback.dummy.invalid;
+
+public class Assertions {
+
+	public static void main() {
+		assert false;
+	}
+	
+}
